Use spin lock impl as the model for locks

src/go_lang/prelude.v
@@ -1,14 +1,12 @@
 From Perennial.go_lang Require Export
-     lang notation slice map struct typing encoding.
+     lang notation slice map struct typing encoding locks.
 
 (* We provide stubs here for primitive operations to make the Goose unit tests
    compile. *)
 
 (* TODO: replace all of these stubs with real operations *)
 
-Inductive LockMode := Reader | Writer.
 Definition uint64_to_string {ext: ext_op}: val := λ: <>, #().
-Definition lockRefT {val_tys: val_types} := refT uint64T.
 Definition strLen {ext: ext_op}: val := λ: "s", #0.
 
 Module Data.
@@ -23,44 +21,6 @@ Module Data.
     Proof.
       typecheck.
     Qed.
-
-    Definition newLock: val := λ: <>, ref #0.
-    Theorem newLock_t: ⊢ newLock : (unitT -> lockRefT).
-    Proof.
-      type_step.
-      type_step.
-      typecheck.
-    Qed.
-
-    Definition lockRelease (m: LockMode): val := λ: <>, #().
-    Theorem lockRelease_t m: ⊢ lockRelease m : (lockRefT -> unitT).
-    Proof.
-      typecheck.
-    Qed.
-
-    Definition lockAcquire (m: LockMode): val := λ: <>, #().
-    Theorem lockAcquire_t m: ⊢ lockAcquire m : (lockRefT -> unitT).
-    Proof.
-      typecheck.
-    Qed.
-
-    (* a cond var is modeled with the underlying lock *)
-    Definition newCondVar: val := λ: "l", (Var "l").
-    (* no-op in the model, only affects scheduling *)
-    Definition condSignal: val := λ: "l", #().
-    Definition condBroadcast: val := λ: "l", #().
-    Definition condWait: val := λ: "l", lockRelease Writer (Var "l");;
-                                        (* actual cond var waits for a signal
-                                        here, but the model does not take this
-                                        into account *)
-                                        lockAcquire Writer (Var "l").
-    (* TODO: prove triples for cond var
-
-       is_cond l I ≜ is_lock l I (* transparent, since caller will continue to use the lock *)
-       {is_lock l I} newCondVar {r. r = l ∗ is_cond r I}
-       {is_cond l I} condSignal l {is_cond l I}
-       {I ∗ is_cond l I} condWait l {I ∗ is_cond l I}
-     *)
   End go_lang.
 End Data.
 
@@ -68,9 +28,6 @@ Hint Resolve Data.stringToBytes_t Data.bytesToString_t : types.
 
 Opaque Data.randomUint64.
 Hint Resolve Data.randomUint64_t : types.
-
-Opaque Data.newLock Data.lockRelease Data.lockAcquire.
-Hint Resolve Data.newLock_t Data.lockRelease_t Data.lockAcquire_t : types.
 
 Module FS.
   Section go_lang.
