src/go_lang/locks.v
@@ -1,0 +1,78 @@
+From Perennial.go_lang Require Import lang notation lib.spin_lock.
+From Perennial.go_lang Require Import lifting.
+From iris.program_logic Require Import weakestpre.
+From Perennial.go_lang Require Import proofmode.
+From Perennial.go_lang Require Import typing.
+Import uPred.
+
+Definition lockRefT {ext} {ext_ty: ext_types ext} := refT boolT.
+
+Module lock.
+  Section go_lang.
+  Context `{ffi_sem: ext_semantics} `{!ffi_interp ffi} `{!heapG Σ} `{!lockG Σ}.
+
+  Local Coercion Var' (s:string) : expr := Var s.
+
+  Definition new := spin_lock.newlock.
+  Definition acquire := spin_lock.acquire.
+  Definition release := spin_lock.release.
+
+  (* a cond var is modeled with the underlying lock *)
+  Definition newCond: val := λ: "l", "l".
+  (* no-op in the model, only affects scheduling *)
+  Definition condSignal: val := λ: "l", #().
+  Definition condBroadcast: val := λ: "l", #().
+  Definition condWait: val := λ: "l", release "l";;
+                                      (* actual cond var waits for a signal
+                                      here, but the model does not take this
+                                      into account *)
+                                      acquire "l".
+
+  Theorem wp_newCond N γ lk R :
+    {{{ is_lock N γ lk R }}}
+      newCond lk
+      {{{ RET lk; is_lock N γ lk R }}}.
+  Proof.
+    iIntros (Φ) "Hl HΦ".
+    wp_call.
+    iApply "HΦ".
+    iFrame.
+  Qed.
+
+  Theorem wp_condSignal N γ lk R :
+    {{{ is_lock N γ lk R }}}
+      condSignal lk
+      {{{ RET #(); is_lock N γ lk R }}}.
+  Proof.
+    iIntros (Φ) "Hc HΦ".
+    wp_call.
+    iApply ("HΦ" with "[$]").
+  Qed.
+
+  Theorem wp_condBroadcast N γ lk R :
+    {{{ is_lock N γ lk R }}}
+      condBroadcast lk
+      {{{ RET #(); is_lock N γ lk R }}}.
+  Proof.
+    iIntros (Φ) "Hc HΦ".
+    wp_call.
+    iApply ("HΦ" with "[$]").
+  Qed.
+
+  Theorem wp_condWait N γ lk R :
+    {{{ is_lock N γ lk R ∗ spin_lock.locked γ ∗ R }}}
+      condWait lk
+      {{{ RET #(); is_lock N γ lk R ∗ spin_lock.locked γ ∗ R }}}.
+  Proof.
+    iIntros (Φ) "(#Hc&Hlocked&HR) HΦ".
+    wp_call.
+    wp_apply (release_spec with "[$Hc $Hlocked $HR]").
+    iIntros "_".
+    wp_pures.
+    wp_apply (acquire_spec with "[$Hc]").
+    iIntros "(Hlocked&HR)".
+    iApply ("HΦ" with "[$]").
+  Qed.
+
+  End go_lang.
+End lock.
